Dafny/LLVM/generalInstructions.i.dfy
@@ -210,7 +210,7 @@ lemma lvm_lemma_Load(lvm_b0:lvm_codes, lvm_s0:lvm_state, lvm_sN:lvm_state,dst:lv
   requires ValidOperand(lvm_s0,dst);
   requires OperandContents(lvm_s0,op1).Ptr?;
   requires MemValid(lvm_s0.m);
-  requires IsValidPtr(lvm_s0.m,OperandContents(lvm_s0,op1).bid,OperandContents(lvm_s0,op1).offset);
+  requires IsValidPtr(lvm_s0.m,OperandContents(lvm_s0,op1).bid,OperandContents(lvm_s0,op1).offset,t);
   // requires lvm_s0.m == lvm_sN.m;
 //   
   ensures  lvm_sM.ok ==> lvm_ensure(lvm_b0, lvm_bM, lvm_s0, lvm_sM, lvm_sN)
@@ -235,7 +235,7 @@ lemma lvm_lemma_Load(lvm_b0:lvm_codes, lvm_s0:lvm_state, lvm_sN:lvm_state,dst:lv
   assert lvm_s0.ok;
   assert ValidInstruction(lvm_s0,lvm_b0.hd.ins);
 
-  assert IsValidPtr(lvm_s0.m, OperandContents(lvm_s0,lvm_b0.hd.ins.src).bid,OperandContents(lvm_s0,lvm_b0.hd.ins.src).offset);
+  assert IsValidPtr(lvm_s0.m, OperandContents(lvm_s0,lvm_b0.hd.ins.src).bid,OperandContents(lvm_s0,lvm_b0.hd.ins.src).offset,t);
 //   assert exists d:Data :: Load(lvm_s0.m,lvm_sN.m,OperandContents(lvm_s0,lvm_b0.hd.ins.src).bid,OperandContents(lvm_s0,lvm_b0.hd.ins.src).offset,d);
   // assert lvm_s0.m == lvm_sN.m;
 //   assert exists d:Data :: Load(lvm_s0.m,lvm_sN.m,OperandContents(lvm_s0,lvm_b0.hd.ins.src).bid,OperandContents(lvm_s0,lvm_b0.hd.ins.src).offset,d); 
